Cslib/Computability/Machines/MultiTapeTuring/Routines/Put.lean
@@ -36,15 +36,9 @@ public def putEnc {k : ℕ} {α : Type*} [StrEnc α] (x : α) (i : Fin k) :
 @[simp]
 public lemma put_eval_struct_empty {k : ℕ} {d : Data} {i : Fin k}
     {views : Fin k → TapeView}
-    (h_empty : (views i).data = Data.list []) :
+    (h_empty : (views i).path = []) :
     (put d i).eval_struct views = some
-      (Function.update views i ⟨d, []⟩) := by sorry
-
-@[simp]
-public lemma put_eval_struct_nonempty {k : ℕ} {d : Data} {i : Fin k}
-    {views : Fin k → TapeView}
-    (h_nonempty : (views i).data ≠ Data.list []) :
-    (put d i).eval_struct views = some views := by sorry
+      (Function.update views i (.ofData d)) := by sorry
 
 end Routines
 end Turing
